\documentclass{article}
\usepackage[margin = 1in]{geometry}
\usepackage{amsmath}
\usepackage{amssymb}

\title{Quadratic Formula}
\author{Stephen Giang}

\begin{document}
	
\maketitle

\begin{align*}
	{ax^{2} + bx + c} = & \enspace 0\\
	x^{2} + \frac{b}{a}x + \frac{c}{a} = & \enspace 0\\
	x^{2} + \frac{b}{a}x + \left( \frac{b}{2a}\right)^{2} + \frac{c}{a} - \left( \frac{b}{2a}\right)^{2}= &\enspace 0\\
	\left( x + \frac{b}{2a} \right)^{2} + \frac{c}{a} - \left( \frac{b}{2a}\right)^{2}= &\enspace 0\\
	\left( x + \frac{b}{2a} \right)^{2} = &-\frac{c}{a} + \left( \frac{b}{2a}\right)^{2}
	\left( x + \frac{b}{2a} \right)^{2} \\
	\left( x + \frac{b}{2a} \right)^{2} = &  \frac{-c}{a} + \frac{b^{2}}{4a^{2}}\\
	\left( x + \frac{b}{2a} \right)^{2} = &  \frac{-4ac}{4a^{2}} + \frac{b^{2}}{4a^{2}}\\
	\left( x + \frac{b}{2a} \right)^{2} = &\enspace \frac{b^{2} - 4ac}{4a^{2}} \\
	\left( x + \frac{b}{2a} \right) = & \enspace\pm \sqrt{\frac{b^{2} - 4ac}{4a^{2}}}\\
	\left( x + \frac{b}{2a} \right) = & \enspace\pm \frac{\sqrt{b^{2} - 4ac}}{2a}\\
	x = & \frac{-b}{2a} \pm \frac{ \sqrt{b^{2} - 4ac}}{2a}\\\\
	x = & \frac{-b \pm \sqrt{b^{2} - 4ac}}{2a}\\
\end{align*}
\begin{center}
	Q.E.D
\end{center}

\end{document}
